## Exercise 1.13
Prove that Fib(n) is the closest integer to $\phi^n$, where $\phi=\frac{1+\sqrt{5}}{2}$. Hint: Let $\psi=\frac{1-\sqrt{5}}{2}$. Use induction and the definition of the Fibonacci numbers (see Section 1.2.2) to prove that $Fib(n)=\frac{1}{\sqrt{5}}(\phi^n-\psi^n)$

**Ans**

证:

令$\psi=\frac{1-\sqrt{5}}{2}$

当 $n=1$ 时有

$Fib(1) = 1$

$\begin{aligned}
\frac{\phi^1-\psi^1}{\sqrt{5}} 
  &= \frac{1}{\sqrt{5}}(\frac{1+\sqrt{5}}{2} - \frac{1-\sqrt{5}}{2}) \\
  &= \frac{1}{2\sqrt{5}}((1 + \sqrt{5})-(1 - \sqrt{5})) \\
  &= \frac{2\sqrt{5}}{2\sqrt{5}} \\
  &= 1 \\
  &= Fib(1)
\end{aligned}$

当 $n=2$ 时有

$Fib(2) = 1$

$\begin{aligned}
\frac{\phi^2-\psi^2}{\sqrt{5}} 
  &= \frac{1}{\sqrt{5}}(\frac{1+\sqrt{5}}{2})^2 - (\frac{1-\sqrt{5}}{2})^2 \\
  &= \frac{1}{\sqrt{5}}(\frac{6 + 2\sqrt{5}}{4}-\frac{6 - 2\sqrt{5}}{4}) \\
  &= \frac{1}{4\sqrt{5}}((6 + 2\sqrt{5})-(6 - 2\sqrt{5})) \\
  &= \frac{4\sqrt{5}}{4\sqrt{5}} \\
  &= 1 \\
  &= Fib(2)
\end{aligned}$

当 $n >= 3$时
假设 $Fib(n-1) = \frac{1}{\sqrt{5}}(\phi^{n-1}-\psi^{n-1})$
及 $Fib(n-2) = \frac{1}{\sqrt{5}}(\phi^{n-2}-\psi^{n-2})$ 成立

$\begin{aligned}
Fib(n) &= Fib(n-1) + Fib(n-2) \\
       &= \frac{1}{\sqrt{5}}(\phi^{n-1}-\psi^{n-1}) + \frac{1}{\sqrt{5}}(\phi^{n-2}-\psi^{n-2}) \\
       &= \frac{1}{\sqrt{5}}((\phi^{n-1} + \phi^{n-2}) - (\psi^{n-1} + \psi^{n-2}) ) \\
       &= \frac{1}{\sqrt{5}}(\phi^{n-2}(1 + \frac{1+\sqrt{5}}{2}) - \psi^{n-2}(1 + \frac{1-\sqrt{5}}{2})) \\
       &= \frac{1}{\sqrt{5}}(\phi^{n-2}\frac{3+\sqrt{5}}{2} - \psi^{n-2}\frac{3-\sqrt{5}}{2}) \\
       &= \frac{1}{\sqrt{5}}(\phi^{n-2}\frac{6+2\sqrt{5}}{4} - \psi^{n-2}\frac{6-2\sqrt{5}}{4}) \\
       &= \frac{1}{\sqrt{5}}(\phi^{n-2}\frac{1+2\sqrt{5}+\sqrt{5}^2}{2^2} - \psi^{n-2}\frac{1-2\sqrt{5}+\sqrt{5}^2}{2^2}) \\
       &= \frac{1}{\sqrt{5}}(\phi^{n-2}(\frac{1+\sqrt{5}}{2})^2 - \psi^{n-2}(\frac{1-\sqrt{5}}{2})^2) \\
       &= \frac{1}{\sqrt{5}}(\phi^{n-2}\phi^2 - \psi^{n-2}\psi^2) \\
       &= \frac{1}{\sqrt{5}}(\phi^n - \psi^n) \\
\end{aligned}$

所以当 $n>=3$ 时有 $Fib(n) = \frac{1}{\sqrt{5}}(\phi^n-\psi^n)$ 成立

$\begin{aligned}
\left|  Fib(n) - \frac{\phi^n}{\sqrt{5}}\right| 
&= \left| \frac{1}{\sqrt{5}}(\phi^n-\psi^n) - \frac{\phi^n}{\sqrt{5}} \right | \\
&= \left|\frac{\psi^n}{\sqrt{5}} \right|\\
&= \left|\frac{1}{\sqrt{5}}(\frac{1-\sqrt{5}}{2})^n\right| \\
&= \frac{1}{\sqrt{5}}(\frac{\sqrt{5}-1}{2})^n \\
&< \frac{1}{\sqrt{5}}(\frac{3-1}{2})^n \\
&< \frac{1}{\sqrt{5}} \\
&< \frac{1}{2} \\
\end{aligned}$

证毕
